int/Intersection.v
@@ -28,933 +28,887 @@ Module Intersection.
       | (S ?m) => feed H ; [| feed_n m H]
     end.
   
-  
-  
-  Section BigSection.
+  (* TODO: del *)
+  Notation "x 'el' A" := (In x A) (at level 70). 
 
-    (* TODO: del *)
-    Notation "x 'el' A" := (In x A) (at level 70). 
+  (** * Util *)
+  (** In this section we prove TODO. *)      
+  Section Util.
+ 
+    Section Proections.
+      
+      Context {A B C: Type}.
+      
+      Definition fst3 (t: A * B * C): A := let '(from, _, _) := t in from.
+      Definition snd3 (t: A * B * C): B := let '(_, r,_) := t in r.
+      Definition thi3 (t: A * B * C): C := let '(_, _, to) := t in to.
+      
+    End Proections.
     
-    Section Util.
-      
-      Section Kek.
+    Section Packing.
+
+      Definition unVar {Vt: Type} (v: @var Vt) := let '(V e) := v in e.
+
+      Section ToWordFunction.
         
-        Lemma ldl:
-          forall (T: eqType) (x: T) A,
-            In x A <-> x \in A.
-        Proof.
-          intros.
-          induction A; first by split.
-          split; intros.
-          { move: H => [H | H].
-            - by subst a; rewrite in_cons; apply/orP; left.
-            - by rewrite in_cons; apply/orP; right; apply IHA.
-          }
-          { move: H; rewrite in_cons; move => /orP [/eqP H | H].
-            - by subst.
-            - by right; apply IHA.
-          }
-        Qed.
-
-      End Kek.
-
-      Section Proections.
-        
-        Context {A B C: Type}.
-        
-        Definition fst3 (t: A * B * C): A := let '(from, _, _) := t in from.
-        Definition snd3 (t: A * B * C): B := let '(_, r,_) := t in r.
-        Definition thi3 (t: A * B * C): C := let '(_, _, to) := t in to.
-        
-      End Proections.
-      
-      Section Packing.
-        
-        Section SEction100.
-          
-          Context {Tt Vt: Type}.
-          
-          Definition unTer (t: ter): Tt := let '(T e) := t in e.
-          Definition unVar (v: var): Vt := let '(V e) := v in e.
-
-        End SEction100.
-      Section Kek.
-
-
-        (* TODO remove duplicate *)
-        Fixpoint to_phrase {T V: Type} (w: word): @phrase T V :=
-          match w with
-            | s::sx => Ts s :: to_phrase sx
-            | _ => []
-          end.
-                
-      End Kek.        
-
-        Section Sec.
-          
-          Context {T V: Type}.
-
-          Fixpoint to_word (p: @phrase T V): list ter :=
-            match p with
-              | Ts x :: sx => x :: to_word sx
-              | _ => []
-            end.
-
-
-          Lemma lemma2: forall (w: word), terminal (@to_phrase T V w).
-          Proof.
-            intros w.
-            induction w.
-            - intros s IN; inversion IN.
-            - intros s IN.
-              inversion IN; auto.
-              subst s; exists a; auto.
-          Qed.
-
-          Lemma lemma3: forall (w: word), to_word (to_phrase w) = w.
-          Proof.
-            intros w.
-            induction w; auto.
-            simpl; rewrite IHw; reflexivity.
-          Qed.
-
-        End Sec.
-
-        Section EqSection.
-
-          Context {T V1 V2: Type}.
-
-          Variable F: V1 -> V2.
-          
-          Definition trans_var v :=
-            V (F (unVar v)).
-          
-          Definition trans_symb symb: @symbol T V2 :=
-            match symb with
-              | Ts t => Ts t
-              | Vs v => Vs (trans_var v)
-            end.
-          
-          Definition trans_phrase p: @phrase T V2 :=
-            map trans_symb p.
-
-        End EqSection.
-        
-      End Packing.
-
-      Section Terminal.
-
         Context {T V: Type}.
 
-        Variable w1 w2: @phrase T V.
+        Fixpoint to_word (phrase: @phrase T V): list ter :=
+          match phrase with
+            | Ts x :: sx => x :: to_word sx
+            | _ => []
+          end.
 
-        Lemma lemma23:
-          terminal w1 ->
-          terminal w2 ->
-          to_word (w1 ++ w2) = to_word w1 ++ to_word w2.
+        (* TODO: name *)
+        Lemma lemma3:
+          forall word, to_word (to_phrase word) = word.
         Proof.
-          intros.
-          induction w1 as [|a w]; auto.
-          destruct a as [t|v]; simpl in *.
-          rewrite IHw; [reflexivity|].
-          intros s EL.
-          apply H; right; exact EL.
-          exfalso.
-          unfold terminal in *.
-          assert(EL: In (Vs v) (Vs v :: w)); auto.
-          destruct  (H _ EL).
-          inversion H1.
-        Qed.
-        
-      End Terminal.
-
-      Section Normalize.
-        
-        (* TODO: comment *)
-        Context {Tt Vt: eqType}.
-
-        (* TODO: comment *)
-        Hypothesis H_T_eq_dec: eq_dec Tt.
-        Hypothesis H_V_eq_dec: eq_dec Vt. 
-
-        (* TODO: comment *)
-        Variable TToNat: Tt -> nat.
-        Variable UToNat: Vt -> nat.
-        Variable NatToU: nat -> Vt.
-        
-        Hypothesis bijection: forall x : nat, UToNat (NatToU x) = x.
-
-        (* Consider an arbitrary grammar  *)
-        Variable G: @grammar Tt Vt.
-
-        (* TODO: comment *)
-        Variable S: @var Vt.
-        Hypothesis H_name: Vs S el dom G.
-
-        (* TODO: comment *)
-        Let normalize G := @normalize Tt Vt _ _ TToNat UToNat NatToU bijection G. 
-        
-        Lemma lflfl:
-          ~ language (normalize G) S [].
-        Proof.
-          intros NLANG.
-          move: NLANG => [DER TER].
-          apply empty_is_not_derivable in DER.
-          - by done.
-          - by apply chomsky_normalform.
+          intros w.
+          induction w; auto.
+          simpl; rewrite IHw; reflexivity.
         Qed.
 
-      End Normalize.
+      End ToWordFunction.
 
-      Section Der.
+      Section EqSection.
 
-        (* TODO: comment *)
-        Hypothesis H_syntactic_analysis: syntactic_analysis_is_possible.
+        Context {T V1 V2: Type}.
+
+        Variable F: V1 -> V2.
         
-        Lemma Fact1: forall Tt Vt a w v, ~ @der Tt Vt [R v []] v (Ts a :: to_phrase w).
-        Proof.
-          unfold syntactic_analysis_is_possible in *.
-          intros ? ? ? ? ? ?.
-          apply H_syntactic_analysis in H.
-          move: H => [H | H].
-          - by inversion H.
-          - move: H => [rhs [EQ DER]].
-            inversion EQ; inversion H; subst; clear H EQ.
-            apply derivability_from_empty in DER.
-              by inversion DER.
-        Qed.
-
-      End Der.
-      
-    End Util.
-
-    Section CanonicalStructureTer.
-      
-      Section EqTer.
+        Definition trans_var v :=
+          V (F (unVar v)).
         
-        Variable T: eqType.
-        
-        Fixpoint eqter (t1 t2: @ter T) :=
-          match t1, t2 with
-            | Definitions.T x1, Definitions.T x2 => x1 == x2
+        Definition trans_symb symb: @symbol T V2 :=
+          match symb with
+            | Ts t => Ts t
+            | Vs v => Vs (trans_var v)
           end.
         
-        Lemma eqterP: Equality.axiom eqter.
-        Proof.
-          move => t1 t2; apply: (iffP idP) => [| <-]; last by elim: t1 => //= t ->.
-          intros; destruct t1, t2.
-            by inversion H as [H']; move: H' => /eqP H'; subst.
-        Defined. 
+        Definition trans_phrase p: @phrase T V2 :=
+          map trans_symb p.
 
-        Global Definition ter_eqMixin := EqMixin eqterP.
-        Canonical ter_eqType := Eval hnf in EqType ter ter_eqMixin.
-
-      End EqTer. 
+      End EqSection.
       
-      Section ChoiceTypeTer.
+    End Packing.
 
-        Variable T: choiceType.
-        
-        Definition to_ter (x: T) := Definitions.T x.
-        Definition from_ter t: T := match t with Definitions.T x => x end.
-        
-        Lemma hz_of_terK : cancel from_ter to_ter.
-        Proof.
-            by intros t; destruct t.
-        Qed.
-        
-        Global Definition ter_choiceMixin := CanChoiceMixin hz_of_terK.
-        Canonical ter_choiceType := Eval hnf in ChoiceType ter ter_choiceMixin.
+    Section TerminalProp.
 
-      End ChoiceTypeTer.
-
-      Section CountTypeTer.
-
-        Variable T: countType.
-        
-        Global Definition ter_countMixin := CanCountMixin (@hz_of_terK T).
-        Canonical ter_countType := Eval hnf in CountType ter ter_countMixin.
-        
-      End CountTypeTer.
-
-      Section FinTypeTer.
-        
-        Variable T: finType.
-        
-        Definition ter_enum := map (@Definitions.T _) (Finite.enum T).
-        
-        Lemma ter_enumP: Finite.axiom ter_enum.
-        Proof.
-          intros x; destruct x as [t].
-            by rewrite //= count_map enumP.
-        Qed.
-        
-        Global Definition ter_finMixin := FinMixin ter_enumP.
-        Canonical ter_finType := Eval hnf in FinType ter ter_finMixin.
-        
-      End FinTypeTer.
-
-    End CanonicalStructureTer.
-    
-    Section SomeSection.
+      Context {T V: Type}.
       
+      Variable word word1 word2: @phrase T V.
+
+      (* TODO: name *)
+      Lemma lemma2:
+        forall word, terminal (@to_phrase T V word).
+      Proof.
+        intros w.
+        induction w.
+        - intros s IN; inversion IN.
+        - intros s IN.
+          inversion IN; auto.
+          subst s; exists a; auto.
+      Qed.       
+
+      (* TODO: name *)
+      Lemma lemma23:
+        terminal word1 ->
+        terminal word2 ->
+        to_word (word1 ++ word2) = to_word word1 ++ to_word word2.
+      Proof.
+        intros.
+        induction word1 as [|a w]; auto.
+        destruct a as [t|v]; simpl in *.
+        rewrite IHw; [reflexivity|].
+        intros s EL.
+        apply H; right; exact EL.
+        exfalso.
+        unfold terminal in *.
+        assert(EL: In (Vs v) (Vs v :: w)); auto.
+        destruct  (H _ EL).
+        inversion H1.
+      Qed.
+
+    End TerminalProp.
+
+    Section Normalize.
+      
+      Context {Tt Vt: eqType}.
+
+      Hypothesis H_T_eq_dec: eq_dec Tt.
+      Hypothesis H_V_eq_dec: eq_dec Vt. 
+
+      Variable TToNat: Tt -> nat.
+      Variable UToNat: Vt -> nat.
+      Variable NatToU: nat -> Vt.
+      
+      Hypothesis bijection: forall x : nat, UToNat (NatToU x) = x.
+
+      (* Consider an arbitrary grammar  *)
+      Variable G: @grammar Tt Vt.
+      Variable S: @var Vt.
+      Hypothesis H_S_el_of_G: Vs S el dom G.
+
       (* TODO: comment *)
-      Variable Tt Vt: Type.
-
-      Section DFAListValues.
-        
-        Fixpoint values_list_gen n: list (t n) :=
-          match n with
-            | O => nil
-            | S n' => F1 :: (map FS (values_list_gen n'))
-          end.     
-        
-        Theorem all_values_in_list:
-          forall (n: nat) (f: t n), f el values_list_gen n.
-        Proof.
-          intros; induction f; [left | right].
-          reflexivity.
-          apply in_map; exact IHf.
-        Qed.
-
-      End DFAListValues.
-
-
-      Variable n: nat.
-      Let DfaState: Type := t n.
-      Let values_list: list DfaState := values_list_gen n.
-
+      Let normalize G := @normalize Tt Vt _ _ TToNat UToNat NatToU bijection G. 
       
-      Section Conversion.
+      Lemma epsilon_is_not_derivable_in_normalized_grammar:
+        ~ language (normalize G) S [].
+      Proof.
+        intros NLANG.
+        move: NLANG => [DER TER].
+        apply empty_is_not_derivable in DER.
+        - by done.
+        - by apply chomsky_normalform.
+      Qed.
 
+    End Normalize.
 
-        Context {T1 T2: Type}.
-        
+    Section EpsilonGrammar.
 
-        
-        
-        Let TripleRule := @rule T1 (DfaState * @var T2 * DfaState).
-        
-        Section ToTriple.
+      Context {Tt Vt: Type}.
 
-          Definition convert_nonterm_rule_2 (r r1 r2: _) (s1 s2 : _): seq.seq TripleRule :=
-            map (fun s3 => R (V (s1, r, s3)) [Vs (V (s1, r1, s2)); Vs (V (s2, r2, s3))]) (values_list).
+      Hypothesis H_syntactic_analysis: syntactic_analysis_is_possible.      
 
-          Definition convert_nonterm_rule_1  (r r1 r2: _) (s1 : _) :=
-            flat_map (convert_nonterm_rule_2 r r1 r2 s1) values_list.
-
-          Definition convert_nonterm_rule (r r1 r2: _) :=
-            flat_map (convert_nonterm_rule_1 r r1 r2) values_list.
-
-          Definition convert_terminal_rule (next: _) (r: _) (t: _): list TripleRule :=
-            map (fun s1 => R (V (s1, r, next s1 t)) [Ts t]) values_list.
-
-          Definition convert_rule (next: _) r :=
-            match r with
-              | R r [Vs r1; Vs r2] => convert_nonterm_rule r r1 r2
-              | R r [Ts t] => convert_terminal_rule next r t 
-              | _  => []
-            end.
-
-        End ToTriple.
-
-        Definition convert_rules (rules: list rule) (next: _): list rule :=
-          flat_map (convert_rule next) rules.
-        
-
-        Definition convert_grammar (g: @grammar _ _) (d: DFA.s_dfa): @grammar _ (_ * @var _ * _):=
-          convert_rules g (DFA.s_next d). 
-
-
-      End Conversion.
-
-      Hint Resolve lemma2.
-
-
-      Section ForwardTerminalRuleInclusion.
-        
-        Variable G: @grammar Tt Vt. 
-        
-        Lemma forward_terminal_rule_inclusion:
-          forall (r: var) (te: ter) (next: _) (from to: DfaState),
-            R r [Ts te] el G ->  
-            next from te = to ->
-
-            R (V (from, r, to)) [Ts te] el convert_rules G next.
-        Proof. 
-          intros r te next from to EL STEP.
-          induction G; [auto | ].
-
-          destruct EL as [EQ | EL].
-          - subst a.
-            apply in_or_app; left; simpl.
-            apply in_map_iff.
-            exists from; subst to.
-            split; [reflexivity | apply all_values_in_list].
-          - simpl.
-            apply in_or_app; right.
-            auto.
-        Qed.
-
-      End ForwardTerminalRuleInclusion.
+      (* Grammar which has only one epsilon rule. *)
+      Variable var: @var Vt.
+      Let epsilon_grammar: @grammar Tt Vt := [R var []].
       
-      Section ForwardNonterminalRuleInclusion.
+      Lemma non_epsilon_is_not_derivable_in_epsilon_grammar:
+        forall ter word,
+          ~ der epsilon_grammar var (Ts ter :: to_phrase word).
+      Proof.
+        unfold syntactic_analysis_is_possible in *.
+        intros ? ? ?.
+        apply H_syntactic_analysis in H.
+        move: H => [H | H].
+        - by inversion H.
+        - move: H => [rhs [EQ DER]].
+          inversion EQ; inversion H; subst; clear H EQ.
+          apply derivability_from_empty in DER.
+            by inversion DER.
+      Qed.
+      
+    End EpsilonGrammar.
+    
+  End Util.
 
-        Variable G: @grammar Tt Vt.
-        Variable next: @dfa_rule DfaState Tt.
-        
 
-        Variable from mid to: DfaState.
-        Variable r r1 r2: @var Vt.
-        
-        Lemma forward_nonterminal_rule_inclusion'':
-          @R Tt _ (V (from, r, to)) [Vs (V(from, r1, mid)); Vs (V (mid, r2, to))] el 
-             convert_nonterm_rule_2 r r1 r2 from mid.
-        Proof.
-          set (rule := (R (V (from, r, to)) [Vs (V(from, r1, mid)); Vs (V (mid, r2, to))])).
-          unfold convert_nonterm_rule_2.
-          set (vals := values_list).
-          assert (H2: to el vals).
-          apply all_values_in_list.  
-          induction vals.
-          simpl in H2.
-          contradiction.
-          simpl.  
-          simpl in H2.
-          destruct H2.
-          left.
-          rewrite H.
+  (** * Canonical structures *)
+  (** In this section we prove TODO. *)
+  Section CanonicalStructureTer.
+    
+    Section EqTer.
+      
+      Variable T: eqType.
+      
+      Fixpoint eqter (t1 t2: @ter T) :=
+        match t1, t2 with
+          | Definitions.T x1, Definitions.T x2 => x1 == x2
+        end.
+      
+      Lemma eqterP: Equality.axiom eqter.
+      Proof.
+        move => t1 t2; apply: (iffP idP) => [| <-]; last by elim: t1 => //= t ->.
+        intros; destruct t1, t2.
+          by inversion H as [H']; move: H' => /eqP H'; subst.
+      Defined. 
+
+      Global Definition ter_eqMixin := EqMixin eqterP.
+      Canonical ter_eqType := Eval hnf in EqType ter ter_eqMixin.
+
+    End EqTer. 
+    
+    Section ChoiceTypeTer.
+
+      Variable T: choiceType.
+      
+      Definition to_ter (x: T) := Definitions.T x.
+      Definition from_ter t: T := match t with Definitions.T x => x end.
+
+      Lemma cancelterK: cancel from_ter to_ter.
+      Proof. by intros t; destruct t. Qed.
+      
+      Global Definition ter_choiceMixin := CanChoiceMixin cancelterK.
+      Canonical ter_choiceType := Eval hnf in ChoiceType ter ter_choiceMixin.
+
+    End ChoiceTypeTer.
+
+    Section CountTypeTer.
+
+      Variable T: countType.
+      
+      Global Definition ter_countMixin := CanCountMixin (@cancelterK T).
+      Canonical ter_countType := Eval hnf in CountType ter ter_countMixin.
+      
+    End CountTypeTer.
+
+    Section FinTypeTer.
+      
+      Variable T: finType.
+      
+      Definition ter_enum := map (@Definitions.T _) (Finite.enum T).
+      
+      Lemma ter_enumP: Finite.axiom ter_enum.
+      Proof.
+        intros x; destruct x as [t].
+          by rewrite //= count_map enumP.
+      Qed.
+      
+      Global Definition ter_finMixin := FinMixin ter_enumP.
+      Canonical ter_finType := Eval hnf in FinType ter ter_finMixin.
+      
+    End FinTypeTer.
+
+  End CanonicalStructureTer.
+
+  (** * Definitions and lemmas *)
+  (** In this section we define a function that creates a intersection-grammar and prove the necessary lemmas. *)
+  Section Lemmas. 
+    
+    (* TODO: comment *)
+    Variable Tt Vt: Type.
+
+    (* TODO: comment *)
+    Section DFAListOfStates.
+      
+      Fixpoint values_list_gen number_of_states: list (t number_of_states) :=
+        match number_of_states with
+          | O => nil
+          | S n' => F1 :: (map FS (values_list_gen n'))
+        end.     
+
+      Theorem all_values_in_list:
+        forall (number_of_states: nat) (state: t number_of_states),
+          state el values_list_gen number_of_states.
+      Proof.
+        intros.
+        induction state; first by left.
+          by right; apply in_map.
+      Qed.
+
+    End DFAListOfStates.
+
+    (* TODO: comment *)
+    Variable number_of_states: nat.
+    Let DfaState: Type := t number_of_states.
+    Let list_of_states: list DfaState := values_list_gen number_of_states.
+
+    (** In this section we define a function that creates a intersection-grammar out of a list of grammars and DFA.  *)
+    Section Conversion.
+
+      Context {T1 T2: Type}.
+      
+      Let TripleRule := @rule T1 (DfaState * @var T2 * DfaState).
+      
+      Definition convert_nonterm_rule_2 (r r1 r2: _) (s1 s2 : _): seq TripleRule :=
+        map (fun s3 => R (V (s1, r, s3)) [Vs (V (s1, r1, s2)); Vs (V (s2, r2, s3))]) list_of_states.
+
+      Definition convert_nonterm_rule_1  (r r1 r2: _) (s1 : _) :=
+        flat_map (convert_nonterm_rule_2 r r1 r2 s1) list_of_states.
+
+      Definition convert_nonterm_rule (r r1 r2: _) :=
+        flat_map (convert_nonterm_rule_1 r r1 r2) list_of_states.
+
+      Definition convert_terminal_rule (next: _) (r: _) (t: _): list TripleRule :=
+        map (fun s1 => R (V (s1, r, next s1 t)) [Ts t]) list_of_states.
+
+      Definition convert_rule (next: _) (r: _ ) :=
+        match r with
+          | R r [Vs r1; Vs r2] => convert_nonterm_rule r r1 r2
+          | R r [Ts t] => convert_terminal_rule next r t 
+          | _  => []
+        end.
+      
+      Definition convert_rules (rules: list rule) (next: _): list rule :=
+        flat_map (convert_rule next) rules.
+      
+      Definition convert_grammar (g: grammar) (d: s_dfa): @grammar _ (_ * _ * _):=
+        convert_rules g (s_next d). 
+
+    End Conversion.
+
+    (** Next, we TODO.  *)    
+    (* In this section we prove that if an initial grammar contains some terminal rule, 
+       then the triple grammar contains the corresponding triple rule. We can simply get
+       the triple rule using application of the "convert_rule" function. *)
+    Section ForwardTerminalRuleInclusion.
+      
+      Variable G: @grammar Tt Vt. 
+      
+      Lemma forward_terminal_rule_inclusion:
+        forall (r: var) (te: ter) (next: _) (from to: DfaState),
+          R r [Ts te] el G ->  
+          next from te = to ->
+          R (V (from, r, to)) [Ts te] el convert_rules G next.
+      Proof. 
+        intros r te next from to EL STEP.
+        induction G; first by done.
+        destruct EL as [EQ | EL].
+        - subst a.
+          apply in_or_app; left; simpl.
+          apply in_map_iff.
+          exists from; subst to.
+          split; [reflexivity | apply all_values_in_list].
+        - simpl.
+          apply in_or_app; right.
           auto.
-          right.
-          apply IHvals.
-          exact H.
-        Qed.
+      Qed.
 
-        Lemma forward_nonterminal_rule_inclusion':
-          @R Tt _ (V (from, r, to)) [Vs (V(from, r1, mid)); Vs (V (mid, r2, to))] el 
-             convert_nonterm_rule_1 r r1 r2 from.
-        Proof.
+    End ForwardTerminalRuleInclusion.
+
+    (* In this section we prove that if an initial grammar contains some nonterminal rule, 
+       then the triple grammar contains the corresponding triple rule. We can simply get
+       the triple rule using application of the "convert_rule" function. *)      
+    Section ForwardNonterminalRuleInclusion.
+
+      Variable G: @grammar Tt Vt.
+      Variable next: @dfa_rule DfaState Tt.
+
+      Variable from mid to: DfaState.
+      Variable r r1 r2: @var Vt.
+
+      Let R := @R Tt.
+      
+      Lemma forward_nonterminal_rule_inclusion'':
+        R (V (from, r, to)) [Vs (V(from, r1, mid)); Vs (V (mid, r2, to))] el 
+          convert_nonterm_rule_2 r r1 r2 from mid.
+      Proof.
+        set (rule := (R (V (from, r, to)) [Vs (V(from, r1, mid)); Vs (V (mid, r2, to))])).
+        unfold convert_nonterm_rule_2.
+        set (vals := list_of_states).
+        assert (H2: to el vals).
+        apply all_values_in_list.  
+        induction vals.
+        simpl in H2.
+        contradiction.
+        simpl.  
+        simpl in H2.
+        destruct H2.
+        left.
+        rewrite H.
+        auto.
+        right.
+        apply IHvals.
+        exact H.
+      Qed.
+
+      Lemma forward_nonterminal_rule_inclusion':
+        R (V (from, r, to)) [Vs (V(from, r1, mid)); Vs (V (mid, r2, to))] el 
+          convert_nonterm_rule_1 r r1 r2 from.
+      Proof.
+        set (rule := (R (V (from, r, to)) [Vs (V(from, r1, mid)); Vs (V (mid, r2, to))])).
+        unfold convert_nonterm_rule_1.
+        set (vals := list_of_states).
+        assert (H2: mid el vals).
+        apply all_values_in_list.
+        induction vals.
+        simpl in H2.
+        contradiction.
+        simpl.  
+        simpl in H2.
+        apply in_or_app. 
+        destruct H2.
+        left.
+        rewrite H. 
+        apply forward_nonterminal_rule_inclusion''.  
+        right. 
+        apply IHvals.
+        apply H.
+      Qed.
+      
+      Lemma forward_nonterminal_rule_inclusion:
+        R r [Vs r1; Vs r2] el G ->
+        R (V (from, r, to)) [Vs (V (from, r1, mid)); Vs (V (mid, r2, to))] el convert_rules G next.
+      Proof.
+        intros EL.
+        induction G; [auto | ].
+        destruct EL as [ | EL]; subst.
+        { clear IHg.
+          apply in_or_app; left; simpl.
           set (rule := (R (V (from, r, to)) [Vs (V(from, r1, mid)); Vs (V (mid, r2, to))])).
-          unfold convert_nonterm_rule_1.
-          set (vals := values_list).
-          assert (H2: mid el vals).
+          unfold convert_nonterm_rule.
+          set (vl := list_of_states).
+          assert (EL: from el vl).
           apply all_values_in_list.
-          induction vals.
-          simpl in H2.
-          contradiction.
-          simpl.  
-          simpl in H2.
-          apply in_or_app. 
-          destruct H2.
-          left.
-          rewrite H. 
-          apply forward_nonterminal_rule_inclusion''.  
-          right. 
-          apply IHvals.
-          apply H.
-        Qed.
-        
-        Lemma forward_nonterminal_rule_inclusion:
-          R r [Vs r1; Vs r2] el G ->
-          R (V (from, r, to)) [Vs (V (from, r1, mid)); Vs (V (mid, r2, to))] el convert_rules G next.
-        Proof.
-          intros EL.
-          induction G; [auto | ].
-          destruct EL as [ | EL]; subst.
-          { clear IHg.
-            apply in_or_app; left; simpl.
-            set (rule := (R (V (from, r, to)) [Vs (V(from, r1, mid)); Vs (V (mid, r2, to))])).
-            unfold convert_nonterm_rule.
-            set (vl := values_list).
-            assert (EL: from el vl).
-            apply all_values_in_list.
-            apply in_flat_map.
-            exists from.
-            split; [exact EL | apply forward_nonterminal_rule_inclusion']. }  
-          { apply in_app_iff; right.
-            apply IHg.
-            exact EL. }
-        Qed.
+          apply in_flat_map.
+          exists from.
+          split; [exact EL | apply forward_nonterminal_rule_inclusion']. }  
+        { apply in_app_iff; right.
+          apply IHg.
+          exact EL. }
+      Qed.
 
-      End ForwardNonterminalRuleInclusion. 
+    End ForwardNonterminalRuleInclusion. 
 
-      Section BackwardRuleInclusion.
+    (* In this section we prove that if a triple grammar contains some rule, 
+       then the initial grammar contains corresponding "single" rule. *)
+    Section BackwardRuleInclusion.
 
-        Variable G: @grammar Tt Vt.
-        Hypothesis H_G_in_chomsky_normal_form: chomsky G.
+      Variable G: @grammar Tt Vt.
+      Hypothesis H_G_in_chomsky_normal_form: chomsky G.
 
-        Variable next: @dfa_rule DfaState Tt.
+      Variable next: @dfa_rule DfaState Tt.
 
-        Let projection (s: @symbol Tt (DfaState * var * DfaState)) : @symbol Tt Vt :=
-          match s with
-            | Vs (V (_, r, _)) => Vs r
-            | Ts (T r) => Ts (T r)
-          end.
+      (* For simplicity, let's define a local name. *)
+      Let projection (s: @symbol Tt (DfaState * var * DfaState)) : @symbol Tt Vt :=
+        match s with
+          | Vs (V (_, r, _)) => Vs r
+          | Ts (T r) => Ts (T r)
+        end.
 
-        Lemma backward_rule_inclusion:
-          forall A l, 
-            R A l el convert_rules G next ->
-            R (snd3 (unVar A)) (map projection l) el G.
-        Proof. 
-          intros.
-          destruct A as [[[from r] to]]; simpl in *.
-          unfold convert_rules in *.
-          apply in_flat_map in H.
-          destruct H as [[r' rhs'] [RIN EL]].
-          unfold convert_rule in *.
-          destruct rhs' as [ | [[t1]|v1] ].
-          - inversion EL.
-          - destruct rhs'.
-            + unfold convert_terminal_rule in *.
-              apply in_map_iff in EL.
-              destruct EL as [s [EQ EL]].
-              inversion EQ; subst; exact RIN.
-            + inversion EL.
-          - destruct rhs' as [ | [ | ]]; try inversion EL.
-            destruct rhs'; try inversion EL.
-            unfold convert_nonterm_rule in EL.
-            apply in_flat_map in EL.
-            destruct EL as [st [_ EL]].
-            unfold convert_nonterm_rule_1 in EL.
-            apply in_flat_map in EL.
-            destruct EL as [st' [_ EL]].
-            unfold convert_nonterm_rule_2 in EL.
+      (* We prove that we can simply project a triple rule into an initial one. *)
+      Lemma backward_rule_inclusion:
+        forall rhs lhs, 
+          R rhs lhs el convert_rules G next ->
+          R (snd3 (unVar rhs)) (map projection lhs) el G.
+      Proof. 
+        intros.
+        destruct rhs as [[[from r] to]]; simpl in *.
+        unfold convert_rules in *.
+        apply in_flat_map in H.
+        destruct H as [[r' rhs'] [RIN EL]].
+        unfold convert_rule in *.
+        destruct rhs' as [ | [[t1]|v1] ].
+        - inversion EL.
+        - destruct rhs'.
+          + unfold convert_terminal_rule in *.
             apply in_map_iff in EL.
-            destruct EL as [st'' [EQ _]].
-            inversion EQ.      
-            subst; simpl; exact RIN.
-        Qed.
-        
-        Corollary backward_terminal_rule_inclusion:
-          forall from r to t, 
-            R (V (from, r, to)) [Ts t] el convert_rules G next ->
-            R r [Ts t] el G.
-        Proof.
-          intros; destruct t as [t].
-          apply backward_rule_inclusion in H; simpl in *; exact H.
-        Qed.
-
-        Corollary backward_nonterminal_rule_inclusion:
-          forall from from1 from2 r r1 r2 to to1 to2, 
-            R (V (from, r, to)) [Vs (V (from1, r1, to1)); Vs (V (from2, r2, to2))]
-              el convert_rules G next ->
-            R r [Vs r1; Vs r2] el G.
-        Proof.
-          intros.
-          apply backward_rule_inclusion in H; simpl in *.
-          exact H.
-        Qed.
-
-      End BackwardRuleInclusion.
-
-      Section RemainsInChomskyNormalForm.
-
-        Variable G: @grammar Tt Vt.
-        Hypothesis H_G_in_chomsky_normal_form: chomsky G.
-
-        Variable next: @dfa_rule DfaState Tt.      
-        
-        Lemma remains_chomsky:
-          chomsky (convert_rules G next).
-        Proof.
-          intros. 
-          destruct H_G_in_chomsky_normal_form as [EF [UN [BIN UF]]].
-          repeat split.
-          { intros v rhs EL CONTR; subst rhs.
-            destruct v as [[[from r] to]].
-            apply backward_rule_inclusion in EL; simpl in *.
-            apply EF in EL.
-            auto. }
-          { intros v rhs EL t TEL.
-            destruct t as [t].
-            unfold Separate.uniform in UN.
-            destruct v as [[[from v] to]].
-            apply backward_rule_inclusion in EL; simpl in *.
-            apply UN with (a := T t) in EL.
-            destruct rhs as [ | [[t'] | []]]; simpl in *.
-            + inversion TEL.
-            + inversion EL; apply map_eq_nil in H1.
-              subst; auto.
-            + inversion EL; apply map_eq_nil in H1.
-              subst.
-              destruct TEL as [TEL | TEL]; inversion TEL.
-            + apply in_map_iff.
-              exists (Ts (T t)); split; auto. }
-          { intros v phs EL.
-            destruct v as [[[from v] to]].
-            apply backward_rule_inclusion in EL.
-            apply BIN in EL.
-            rewrite map_length in EL.
-            auto. }
-          { intros v CONTR.
-            destruct v as [[[from r] to]].
-            destruct CONTR as [[[[from' r'] to']] EL].
-            apply backward_rule_inclusion in EL; simpl in *.
-            unfold ElimU.unitfree in *.
-            eapply UF.
-            exists r'.
-            eauto. }
-        Qed.
-
-      End RemainsInChomskyNormalForm.  
-      
-      Section MiddleLemmas.
-
-        Variable G: @grammar Tt Vt.
-        Variable next: @dfa_rule DfaState Tt.
-
-        Lemma middle_lemma_nonterm:
-          forall from from1 from2 r r1 r2 to to1 to2,
-            R (V (from, r, to)) [Vs (V (from1, r1, to1)); Vs (V (from2, r2, to2))]
-              el convert_rules G next ->
-            from = from1 /\ to1 = from2 /\ to = to2.
-        Proof.
-          intros r r1 r2 from from1 from2 to to1 to2 EL.
-          unfold convert_rules in EL.
+            destruct EL as [s [EQ EL]].
+            inversion EQ; subst; exact RIN.
+          + inversion EL.
+        - destruct rhs' as [ | [ | ]]; try inversion EL.
+          destruct rhs'; try inversion EL.
+          unfold convert_nonterm_rule in EL.
           apply in_flat_map in EL.
-          destruct EL as [rule [_ EL]].
-          destruct rule as [v rhs].
-
-          destruct rhs; simpl in *. contradiction.
-          destruct s; simpl in *.
-          { destruct rhs; [| inversion EL].
-            unfold convert_terminal_rule in *.
-            apply in_map_iff in EL; destruct EL as [st [EQ _]]; inversion EQ. }
-          { destruct rhs; [inversion EL | ].
-            destruct s; [ inversion EL | ].
-            destruct rhs; [ | inversion EL].
-            unfold convert_nonterm_rule in EL.
-            unfold convert_nonterm_rule_1 in EL.
-            unfold convert_nonterm_rule_2 in EL.
-            apply in_flat_map in EL. destruct EL as [st1 [_ EL]].
-            apply in_flat_map in EL; destruct EL as [st2 [_ EL]].
-            apply in_map_iff in EL; destruct EL as [st3 [EQ _]].
-            inversion EQ; subst; auto. }
-        Qed.
-
-        Lemma middle_lemma_term:
-          forall from r to te,
-            R (V (from, r, to)) [Ts te] el convert_rules G next ->
-            next from te = to.
-        Proof.
-          intros r from to te EL.
-          unfold convert_rules in EL.
+          destruct EL as [st [_ EL]].
+          unfold convert_nonterm_rule_1 in EL.
           apply in_flat_map in EL.
-          destruct EL as [rule [_ EL]].
-          destruct rule as [v rhs].
-          destruct rhs; simpl in *. contradiction.
-          destruct s; simpl in *.
-          { destruct rhs; [| inversion EL].
-            unfold convert_terminal_rule in *.
-            apply in_map_iff in EL; destruct EL as [st [EQ _]]; inversion EQ; auto. }
-          { destruct rhs; [inversion EL | ].
-            destruct s; [ inversion EL | ].
-            destruct rhs; [ | inversion EL].
-            unfold convert_nonterm_rule in EL.
-            unfold convert_nonterm_rule_1 in EL.
-            unfold convert_nonterm_rule_2 in EL.
-            apply in_flat_map in EL. destruct EL as [st1 [_ EL]].
-            apply in_flat_map in EL; destruct EL as [st2 [_ EL]].
-            apply in_map_iff in EL; destruct EL as [st3 [EQ _]].
-            inversion EQ; subst; auto. }
-        Qed.
-        
-        Corollary middle_lemma_nonterm':
-          forall r r1 r2,
-            R (V r) [Vs (V r1); Vs (V r2)] el convert_rules G next ->
-            fst3 r = fst3 r1 /\ thi3 r1 = fst3 r2 /\ thi3 r = thi3 r2.
-        Proof.
-          intros.
-          destruct r as [[from r] to].
-          destruct r1 as [[from1 r1] to1].
-          destruct r2 as [[from2 r2] to2].
-          simpl in *.
-          eapply middle_lemma_nonterm; eauto.
-        Qed.
-        
-        Corollary middle_lemma_term':
-          forall (r : _) (te : ter),
-            R (V r) [Ts te] el (convert_rules G next) ->
-            next (fst3 r) te = thi3 r.
-        Proof.
-          intros r te H0.
-          destruct r as [[from0 r0] to0].
-          simpl in *.
-          eapply middle_lemma_term; eauto.
-        Qed.
-
-        
-      End MiddleLemmas.
+          destruct EL as [st' [_ EL]].
+          unfold convert_nonterm_rule_2 in EL.
+          apply in_map_iff in EL.
+          destruct EL as [st'' [EQ _]].
+          inversion EQ.      
+            by subst; simpl.
+      Qed.
       
-      Section Main.
+      Corollary backward_terminal_rule_inclusion:
+        forall from r to t, 
+          R (V (from, r, to)) [Ts t] el convert_rules G next ->
+          R r [Ts t] el G.
+      Proof.
+        intros; destruct t as [t].
+        apply backward_rule_inclusion in H; simpl in *; exact H.
+      Qed.
 
-        Variable G: @grammar Tt Vt.
-        Hypothesis H_G_in_chomsky_normal_form: chomsky G.
-        Hypothesis H_syntactic_analysis: syntactic_analysis_is_possible. 
+      Corollary backward_nonterminal_rule_inclusion:
+        forall from from1 from2 r r1 r2 to to1 to2, 
+          R (V (from, r, to)) [Vs (V (from1, r1, to1)); Vs (V (from2, r2, to2))]
+            el convert_rules G next ->
+          R r [Vs r1; Vs r2] el G.
+      Proof.
+          by intros; apply backward_rule_inclusion in H.
+      Qed.
+
+    End BackwardRuleInclusion.
+
+    (* In this section, we prove that after transformation grammar remains in chomsky normal form. *)
+    Section RemainsInChomskyNormalForm.
+
+      Variable G: @grammar Tt Vt.
+      Hypothesis H_G_in_chomsky_normal_form: chomsky G.
+
+      Variable next: @dfa_rule DfaState Tt.      
+
+      (* TODO: explain? *)
+      Lemma remains_chomsky:
+        chomsky (convert_rules G next).
+      Proof.
+        destruct H_G_in_chomsky_normal_form as [EF [UN [BIN UF]]].
+        repeat split.
+        { intros v rhs EL CONTR; subst rhs.
+          destruct v as [[[from r] to]].
+          apply backward_rule_inclusion in EL; simpl in *.
+            by apply EF in EL.
+        }
+        { intros v rhs EL t TEL.
+          destruct t as [t].
+          unfold Separate.uniform in UN.
+          destruct v as [[[from v] to]].
+          apply backward_rule_inclusion in EL; simpl in *.
+          apply UN with (a := T t) in EL.
+          destruct rhs as [ | [[t'] | []]]; simpl in *.
+          + by inversion TEL.
+          + inversion EL; apply map_eq_nil in H1.
+              by subst; auto.
+          + inversion EL; apply map_eq_nil in H1.
+            subst.
+              by destruct TEL as [TEL | TEL]; inversion TEL.
+          + apply in_map_iff.
+              by exists (Ts (T t)); split; auto. }
+        { intros v phs EL.
+          destruct v as [[[from v] to]].
+          apply backward_rule_inclusion in EL.
+          apply BIN in EL.
+            by rewrite map_length in EL.
+        }
+        { intros v CONTR.
+          destruct v as [[[from r] to]].
+          destruct CONTR as [[[[from' r'] to']] EL].
+          apply backward_rule_inclusion in EL; simpl in *.
+          unfold ElimU.unitfree in *.
+          eapply UF.
+            by exists r'; eauto. }
+      Qed.
+
+    End RemainsInChomskyNormalForm.  
+
+    (* In this section, we prove that the triple-rules have certain consistent structure. *)
+    Section ConsistensyOfTripleRules.
+
+      Variable G: @grammar Tt Vt.
+      Variable next: @dfa_rule DfaState Tt. (* TODO: name *)
+
+      Lemma consistensy_of_triple_nonterm_rules:
+        forall from from1 from2 r r1 r2 to to1 to2,
+          R (V (from, r, to)) [Vs (V (from1, r1, to1)); Vs (V (from2, r2, to2))]
+            el convert_rules G next ->
+          from = from1 /\ to1 = from2 /\ to = to2.
+      Proof.
+        intros r r1 r2 from from1 from2 to to1 to2 EL.
+        unfold convert_rules in EL.
+        apply in_flat_map in EL.
+        destruct EL as [rule [_ EL]].
+        destruct rule as [v rhs].
+        destruct rhs; simpl in *; first by done.
+        destruct s; simpl in *.
+        { destruct rhs; [| inversion EL].
+          unfold convert_terminal_rule in *.
+          apply in_map_iff in EL; destruct EL as [st [EQ _]]; inversion EQ. }
+        { destruct rhs; [inversion EL | ].
+          destruct s; [ inversion EL | ].
+          destruct rhs; [ | inversion EL].
+          unfold convert_nonterm_rule in EL.
+          unfold convert_nonterm_rule_1 in EL.
+          unfold convert_nonterm_rule_2 in EL.
+          apply in_flat_map in EL. destruct EL as [st1 [_ EL]].
+          apply in_flat_map in EL; destruct EL as [st2 [_ EL]].
+          apply in_map_iff in EL; destruct EL as [st3 [EQ _]].
+          inversion EQ; subst; auto. }
+      Qed.
+
+      Lemma consistensy_of_triple_term_rules:
+        forall from r to te,
+          R (V (from, r, to)) [Ts te] el convert_rules G next ->
+          next from te = to.
+      Proof.
+        intros r from to te EL.
+        unfold convert_rules in EL.
+        apply in_flat_map in EL.
+        destruct EL as [rule [_ EL]].
+        destruct rule as [v rhs].
+        destruct rhs; simpl in *. contradiction.
+        destruct s; simpl in *.
+        { destruct rhs; [| inversion EL].
+          unfold convert_terminal_rule in *.
+          apply in_map_iff in EL; destruct EL as [st [EQ _]]; inversion EQ; auto. }
+        { destruct rhs; [inversion EL | ].
+          destruct s; [ inversion EL | ].
+          destruct rhs; [ | inversion EL].
+          unfold convert_nonterm_rule in EL.
+          unfold convert_nonterm_rule_1 in EL.
+          unfold convert_nonterm_rule_2 in EL.
+          apply in_flat_map in EL. destruct EL as [st1 [_ EL]].
+          apply in_flat_map in EL; destruct EL as [st2 [_ EL]].
+          apply in_map_iff in EL; destruct EL as [st3 [EQ _]].
+          inversion EQ; subst; auto. }
+      Qed.
+      
+      Corollary consistensy_of_triple_nonterm_rules':
+        forall r r1 r2,
+          R (V r) [Vs (V r1); Vs (V r2)] el convert_rules G next ->
+          fst3 r = fst3 r1 /\ thi3 r1 = fst3 r2 /\ thi3 r = thi3 r2.
+      Proof.
+        intros.
+        destruct r as [[from r] to].
+        destruct r1 as [[from1 r1] to1].
+        destruct r2 as [[from2 r2] to2].
+        simpl in *.
+        eapply consistensy_of_triple_nonterm_rules; eauto.
+      Qed.
+      
+      Corollary consistensy_of_triple_term_rules':
+        forall (r : _) (te : ter),
+          R (V r) [Ts te] el (convert_rules G next) ->
+          next (fst3 r) te = thi3 r.
+      Proof.
+        intros r te H0.
+        destruct r as [[from0 r0] to0].
+        simpl in *.
+        eapply consistensy_of_triple_term_rules; eauto.
+      Qed.
+      
+    End ConsistensyOfTripleRules.
+
+    (** * TODO: name *)
+    (** TODO: comment *)
+    Section Main.
+
+      Variable G: @grammar Tt Vt.
+      Hypothesis H_G_in_chomsky_normal_form: chomsky G.
+      Hypothesis H_syntactic_analysis: syntactic_analysis_is_possible. 
+      
+      Hypothesis F1: DfaState * @var Vt * DfaState -> Vt.
+      Hypothesis F2: Vt -> DfaState * @var Vt * DfaState.
+
+      (** TODO: comment *)
+      Section MainForward.
+
+        (* TODO: comment *)
+        Theorem der_in_initial_grammar_and_dfa_implies_der_in_triple_grammar:
+          forall (next: dfa_rule) (r: var) (from to: DfaState) (word: _),
+            der G r (to_phrase word) ->
+            final_state next from word = to ->
+            der (convert_rules G next) (V (from, r, to)) (to_phrase word).
+        Proof.
+          intros next r from to w DER FIN.          
+          rewrite <- (@lemma3 Tt Vt w) in FIN.
+          set (wp1 := to_phrase (T:=Tt) (V:= _ * @var Vt * _) w) in *.
+          set (wp2 := trans_phrase F2 (to_phrase w)) in *.
+          assert (D: wp1 = wp2).
+          { clear; induction w; simpl in *.
+            reflexivity.
+            unfold wp1, wp2.
+            rewrite <- IHw; auto. }
+          rewrite D; clear D.
+          generalize dependent FIN. 
+          generalize dependent from.
+          generalize dependent to.
+          generalize dependent next.
+          apply chomsky_derivability_induction with 
+          (P := fun r phr =>
+                  forall (next : dfa_rule) (from to : DfaState),
+                    final_state next from (to_word phr) = to ->
+                    der (convert_rules G next) (V (from, r, to)) (trans_phrase F2 phr)) in DER; auto.
+          { intros r0 t IN next from to FIN; simpl in *.
+              by apply rDer, forward_terminal_rule_inclusion; auto. }
+          { intros r0 r1 r2 w1 w2 IN Ind1 Ind2 TER1 TER2 DER1 DER2 next from to FIN0.
+            set (newG := convert_rules G next).
+            set (m := final_state next from (to_word w1)).
+            assert (H1: der newG (V (from, r1, m)) (trans_phrase F2 w1)); eauto.
+            assert (H2: der newG (V (m, r2, to)) (trans_phrase F2 w2)).
+            { apply Ind2, test0.
+              rewrite <- lemma23; auto. }
+            assert (in_H: In (R (V (from, r0, to)) [Vs (V(from, r1, m)); Vs (V (m, r2, to))]) newG).
+            { apply forward_nonterminal_rule_inclusion; auto. }
+            unfold trans_phrase.
+            rewrite map_cat.
+              by eapply derivability_step; eauto. }
+          { by apply lemma2. }
+        Qed.
+
+        (* TODO: comment *)
+        Theorem main_forward:
+          forall sdfa var word,
+            (s_dfa_language sdfa) word /\ language G var (to_phrase word) ->
+            (language (convert_grammar G sdfa) (V (s_start sdfa, var, s_final sdfa)) (to_phrase word)).
+        Proof.
+          intros ? ? ? INT.
+          destruct INT as [DFA [DER TER]].
+            by split; [apply der_in_initial_grammar_and_dfa_implies_der_in_triple_grammar | apply lemma2].
+        Qed.
         
-        Hypothesis F1: DfaState * @var Vt * DfaState -> Vt.
-        Hypothesis F2: Vt -> DfaState * @var Vt * DfaState.
+      End MainForward.
 
-        Section MainForward.
+      (** TODO: comment *)
+      Section MainBackward.
 
-          Theorem der_in_initial_grammar_and_dfa_implies_der_in_triple_grammar:
-            forall (next: dfa_rule) (r: var) (from to: DfaState) (w: word),
-              der G r (to_phrase w) ->
-              final_state next from w = to ->
-              der (convert_rules G next) (V (from, r, to)) (to_phrase w).
+        (* TODO: comment *)
+        Section DerivabilityInTripleGrammarImpliesAcceptanceInDFA.
+
+          Variable next: @dfa_rule DfaState Tt.
+          Variable from to: DfaState.
+          
+          Lemma der_in_triple_grammar_implies_dfa_accepts':
+            forall var word,           
+              der (convert_rules G next) (V (from, var, to)) (to_phrase word) ->     
+              final_state next (fst3 (from, var, to)) word = thi3 (from, var, to).
+          Proof. 
+            intros r w H.
+            assert (EQ: w = to_word (to_phrase(T:=Tt) (V:=DfaState * @var Vt * DfaState) w)).
+            { clear.
+              induction w; simpl.
+              - reflexivity.
+              - rewrite <- IHw; reflexivity.
+            } rewrite EQ; clear EQ.
+            assert (P1: fst3 (from, r, to) = fst3 (unVar (V (from, r, to)))). simpl; reflexivity.
+            assert (P2: thi3 (from, r, to) = thi3 (unVar (V (from, r, to)))). simpl; reflexivity.
+            rewrite P1; rewrite P2; clear P1 P2.
+            apply chomsky_derivability_induction
+            with (w0 := to_phrase w) (r0 := V (from, r, to)) (G0 := convert_rules G next); auto; simpl.
+            { apply remains_chomsky; auto. }
+            { clear H r.
+              intros. 
+              eapply consistensy_of_triple_term_rules'.
+              destruct r; eauto. }
+            { clear H r from to. 
+              intros r r1 r2 w1 w2 IN FIN1 FIN2 TER1 TER2 DER1 DER2.
+              rewrite lemma23; auto.
+              apply test0_1.
+              destruct r as [[[fr r] to]].
+              destruct r1 as [[[fr1 r1] to1]].
+              destruct r2 as [[[fr2 r2] to2]].
+              simpl in *.      
+              assert (EQ:= @consistensy_of_triple_nonterm_rules' G next (fr, r, to) (fr1, r1, to1) (fr2, r2, to2) IN).
+              destruct EQ as [EQ1 [EQ2 EQ3]]; simpl in *.
+              subst fr to1 to2.
+                by rewrite EQ2 EQ3. }
+            { by apply lemma2. }
+          Qed.
+
+          Lemma der_in_triple_grammar_implies_dfa_accepts:
+            forall var word,
+              der (convert_rules G next) (V (from, var , to)) (to_phrase word) ->
+              final_state next from word = to.
           Proof.
-            intros next r from to w DER FIN.          
-            rewrite <- (@lemma3 Tt Vt w) in FIN.
-            set (wp1 := to_phrase (T:=Tt) (V:= _ * @var Vt * _) w) in *.
-            set (wp2 := trans_phrase F2 (to_phrase w)) in *.
-            assert (D: wp1 = wp2).
-            { clear; induction w; simpl in *.
-              reflexivity.
-              unfold wp1, wp2.
-              rewrite <- IHw; auto. }
-            rewrite D; clear D.
+            intros w r DER. 
+            set (rule := (from, r, to)) in *.
+            assert (H1: from = fst3 rule); auto.
+            assert (H2: to = thi3 rule); auto.
+            rewrite H1 H2.
+            eapply der_in_triple_grammar_implies_dfa_accepts'; eauto 1.
+          Qed.
+          
+        End DerivabilityInTripleGrammarImpliesAcceptanceInDFA.
 
-            generalize dependent FIN.
-            generalize dependent from.
-            generalize dependent to.
-            generalize dependent next.
-            
-            apply chomsky_derivability_induction with 
-            (P :=
-               fun r phr =>
-                 forall (next : dfa_rule) (from to : DfaState),
-                   final_state next from (to_word phr) = to ->
-                   der (convert_rules G next) (V (from, r, to)) (trans_phrase F2 phr)
-            ) in DER; auto.
-            { intros r0 t IN next from to FIN; simpl in *.
-              apply rDer, forward_terminal_rule_inclusion; auto. }
-            { intros r0 r1 r2 w1 w2 IN Ind1 Ind2 TER1 TER2 DER1 DER2 next from to FIN0.
-              set (newG := convert_rules G next).
-              set (m := final_state next from (to_word w1)).
-              assert (H1: der newG (V (from, r1, m)) (trans_phrase F2 w1)); eauto.
-              assert (H2: der newG (V (m, r2, to)) (trans_phrase F2 w2)).
-              { apply Ind2, test0.
-                rewrite <- lemma23; auto. }
-              assert (in_H: In (R (V (from, r0, to)) [Vs (V(from, r1, m)); Vs (V (m, r2, to))]) newG).
-              { apply forward_nonterminal_rule_inclusion; auto. }
+        (* TODO: comment *)
+        Section DerivabilityInTripleGrammarImpliesDerivabilityInInitialGrammar.
+
+          Variable next: @dfa_rule DfaState Tt.
+          
+          Lemma der_in_triple_gr_implies_der_in_initial_gr':
+            forall (r: var) word,
+              der (convert_rules G next) r (to_phrase word) ->
+              der G (snd3 (unVar r)) (to_phrase word). 
+          Proof.
+            intros r w H.
+            assert (EQ: trans_phrase F1 (to_phrase  w) = to_phrase w).
+            { clear.
+              induction w; simpl.
+              - reflexivity.
+              - rewrite IHw. reflexivity. }
+            rewrite <- EQ.
+            apply chomsky_derivability_induction with (G0 := convert_rules G next) (r0 := r) (w0 := to_phrase w); auto.
+            { apply remains_chomsky; auto. }
+            { intros r' t IN.
+              destruct r' as [[[from r'] to]]; simpl in *.
+              apply rDer; apply backward_terminal_rule_inclusion in IN; auto. }
+            { intros r' r1 r2 w1 w2 IN DER1 DER2 TER1 TER2 DER3 DER4.
+              destruct r' as [[[from r'] to]].
+              destruct r1 as [[[from1 r1] to1]].
+              destruct r2 as [[[from2 r2] to2]]; simpl in *.
               unfold trans_phrase.
               rewrite map_cat.
-              eapply derivability_step; eauto. }
-
-          Qed.
-
-          Theorem main_forward:
-            forall (d : s_dfa) (v: var) (w : word),
-              (s_dfa_language d) w /\ language G v (to_phrase w) ->
-              (language (convert_grammar G d) (V (s_start d, v, s_final d)) (to_phrase w)).
-          Proof.
-            intros ? ? ? INT.
-            destruct INT as [DFA [DER TER]].
-            split; [apply der_in_initial_grammar_and_dfa_implies_der_in_triple_grammar | ]; auto.
+              apply @derivability_step with (r1 := r1) (r2 := r2) (T := Tt) (V := Vt); auto.
+                by apply backward_nonterminal_rule_inclusion in IN. }
+            { by apply lemma2. }
           Qed.
           
-        End MainForward.
-        
-        Section MainBackward.
-          
-          Section SEction1.
-
-            Variable next: @dfa_rule DfaState Tt.
-            Variable from to: DfaState.
-            
-            Lemma der_in_triple_grammar_implies_dfa_accepts':
-              forall (r : var) (w : word),           
-                der (convert_rules G next) (V (from, r, to)) (to_phrase w) ->     
-                final_state next (fst3 (from, r, to)) w = thi3 (from, r, to).
-            Proof. 
-              intros.
-              assert (EQ: w = to_word (to_phrase(T:=Tt) (V:=DfaState * @var Vt * DfaState) w)).
-              { clear.
-                induction w; simpl.
-                - reflexivity.
-                - rewrite <- IHw; reflexivity.
-              } rewrite EQ; clear EQ.
-              
-              assert (P1: fst3 (from, r, to) = fst3 (unVar (V (from, r, to)))). simpl; reflexivity.
-              assert (P2: thi3 (from, r, to) = thi3 (unVar (V (from, r, to)))). simpl; reflexivity.
-              rewrite P1; rewrite P2; clear P1 P2.
-              
-              apply chomsky_derivability_induction
-              with (w0 := to_phrase w) (r0 := V (from, r, to)) (G0 := convert_rules G next); auto; simpl.
-              { apply remains_chomsky; auto. }
-              { clear H r.
-                intros. 
-                eapply middle_lemma_term'.
-                destruct r; eauto. }
-              { clear H r from to. 
-                intros r r1 r2 w1 w2 IN FIN1 FIN2 TER1 TER2 DER1 DER2.
-                rewrite lemma23; auto.
-                apply test0_1.
-                
-                destruct r as [[[fr r] to]].
-                destruct r1 as [[[fr1 r1] to1]].
-                destruct r2 as [[[fr2 r2] to2]].
-                simpl in *.      
-                
-                assert (EQ:= @middle_lemma_nonterm' G next (fr, r, to) (fr1, r1, to1) (fr2, r2, to2) IN).
-                destruct EQ as [EQ1 [EQ2 EQ3]]; simpl in *.
-                subst fr to1 to2.
-                rewrite EQ2 EQ3; reflexivity. }
-            Qed.
-
-            Lemma der_in_triple_grammar_implies_dfa_accepts:
-              forall (r: var) (w: word),
-                der (convert_rules G next) (V (from, r , to)) (to_phrase w) ->
-                final_state next from w = to.
-            Proof.
-              intros w r DER. 
-              set (rule := (from, r, to)) in *.
-              assert (H1: from = fst3 rule); auto.
-              assert (H2: to = thi3 rule); auto.
-              rewrite H1 H2.
-              eapply der_in_triple_grammar_implies_dfa_accepts'; eauto 1.
-            Qed.
-            
-          End SEction1.
-
-          Section Section2.
-
-            Variable next: @dfa_rule DfaState Tt.
-            
-            Lemma der_in_triple_gr_implies_der_in_initial_gr':
-              forall (r: var) (w: word),
-                der (convert_rules G next) r (to_phrase w) ->
-                der G (snd3 (unVar r)) (to_phrase w). 
-            Proof.
-              intros.
-              assert (EQ: trans_phrase F1 (to_phrase  w) = to_phrase w).
-              { clear.
-                induction w; simpl.
-                - reflexivity.
-                - rewrite IHw. reflexivity. }
-              rewrite <- EQ.
-
-              apply chomsky_derivability_induction with (G0 := convert_rules G next) (r0 := r) (w0 := to_phrase w); auto.
-              { apply remains_chomsky; auto. }
-              { intros r' t IN.
-                destruct r' as [[[from r'] to]]; simpl in *.
-                apply rDer; apply backward_terminal_rule_inclusion in IN; auto. }
-              { intros r' r1 r2 w1 w2 IN DER1 DER2 TER1 TER2 DER3 DER4.
-                destruct r' as [[[from r'] to]].
-                destruct r1 as [[[from1 r1] to1]].
-                destruct r2 as [[[from2 r2] to2]]; simpl in *.
-                unfold trans_phrase.
-                rewrite map_cat.
-                apply @derivability_step with (r1 := r1) (r2 := r2) (T := Tt) (V := Vt); auto.
-                apply backward_nonterminal_rule_inclusion in IN; auto. }
-            Qed.
-            
-            Lemma der_in_triple_gr_implies_der_in_initial_gr:
-              forall (s_start s_final: DfaState)
-                (grammar_start : _) 
-                (w : word),  
-                der (convert_rules G next) (V (s_start, grammar_start, s_final)) (to_phrase w) ->
-                der G grammar_start (to_phrase w).
-            Proof.
-              intros start final g_start w.
-              set (s := (start, g_start, final)).
-              assert (g_start = snd3 s); auto.
-              rewrite H.
-              eapply der_in_triple_gr_implies_der_in_initial_gr'.  
-            Qed.  
-
-            
-
-          End Section2.
-
-          Theorem main_backward:
-            forall (d : s_dfa) (w : @word Tt) (v: var),
-              language (convert_grammar G d) (V (s_start d, v, s_final d)) (to_phrase w) ->
-              s_dfa_language d w /\ language G v (to_phrase w).
+          Lemma der_in_triple_gr_implies_der_in_initial_gr:
+            forall (s_start s_final: DfaState) (grammar_start : _) (w : word),  
+              der (convert_rules G next) (V (s_start, grammar_start, s_final)) (to_phrase w) ->
+              der G grammar_start (to_phrase w).
           Proof.
-            intros ? ? ? TR.
-            destruct TR as [DER TER]. 
-            unfold convert_grammar in DER.
-            destruct d; simpl in *.
-            split.
-            unfold s_dfa_language, s_accepts; simpl.
-            eapply der_in_triple_grammar_implies_dfa_accepts; eauto 1.
-            split.
-            eapply der_in_triple_gr_implies_der_in_initial_gr; eauto 1.
-            auto.
-          Qed.
+            intros start final g_start w.
+            set (s := (start, g_start, final)).
+            assert (g_start = snd3 s); auto.
+            rewrite H.
+            eapply der_in_triple_gr_implies_der_in_initial_gr'.  
+          Qed.  
 
-        End MainBackward. 
-        
-      End Main.
+        End DerivabilityInTripleGrammarImpliesDerivabilityInInitialGrammar.
 
-    End SomeSection.
+        (* Now we can split the conclusion of the lemma and use the lemmas above to finish the proof. *)
+        Theorem main_backward:
+          forall sdfa var word,
+            language (convert_grammar G sdfa) (V (s_start sdfa, var, s_final sdfa)) (to_phrase word) ->
+            s_dfa_language sdfa word /\ language G var (to_phrase word).
+        Proof.
+          intros ? ? ? TR.
+          destruct TR as [DER TER]. 
+          unfold convert_grammar in DER.
+          destruct sdfa; simpl in *.
+          split.
+          unfold s_dfa_language, s_accepts; simpl.
+          eapply der_in_triple_grammar_implies_dfa_accepts; eauto 1.
+          split.
+          - by eapply der_in_triple_gr_implies_der_in_initial_gr; eauto 1.
+          - by apply lemma2.
+        Qed.
 
+      End MainBackward. 
+      
+    End Main.
+
+  End Lemmas.
+  
+  (** * Main Theorem *)
+  (** In this section we prove TODO. *)  
+  Section Main.
     
-  End BigSection.
-
-  (* TODO: comment *)
-  Section Main3.
-    
-    (* TODO: comment *)
-    Context {Tt Vt: eqType}.
+    Context {Terminal Nonterminal: eqType}.
 
     (* TODO: comment *)
-    Hypothesis H_T_eq_dec: eq_dec Tt.
-    Hypothesis H_V_eq_dec: eq_dec Vt.
+    Hypothesis H_T_eq_dec: eq_dec Terminal.
+    Hypothesis H_V_eq_dec: eq_dec Nonterminal.
 
     (* TODO: comment *)
-    Variables (TToNat: Tt -> nat) (UToNat: Vt -> nat) (NatToU: nat -> Vt).
+    Variables (TToNat: Terminal -> nat) (UToNat: Nonterminal -> nat) (NatToU: nat -> Nonterminal).
     Hypothesis bijection: forall x : nat, UToNat (NatToU x) = x.
 
-     
     (* TODO: comment *)
     Hypothesis H_syntactic_analysis: syntactic_analysis_is_possible.
-
     
     (* TODO: comment *)
-    Variable n: nat.
+    Variable number_of_states: nat.
+    Let DfaState: Type := t number_of_states.
+    Let list_of_states: list DfaState := values_list_gen number_of_states.
 
     (* TODO: comment *)
-    Let DfaState: Type := t n.
-    Let values_list: list DfaState := values_list_gen n.
+    Variable dfa: @dfa DfaState Terminal. 
+
+    (* Consider an arbitrary grammar G with start symbol S. *)
+    Variable G: @grammar Terminal Nonterminal.
+    Variable S: @var Nonterminal.
+    Hypothesis H_S_el_of_G: Vs S el dom G.
 
     (* TODO: comment *)
-    Variable dfa: @dfa DfaState Tt. 
-
-
-    (* Consider an arbitrary grammar with start symbol S. *)
-    Variable G: @grammar Tt Vt.
-    Variable S: @var Vt.
-    Hypothesis H_name: Vs S el dom G.
-
-    (* TODO: comment *)
-    Lemma grammar_of_intersection_exists:
-      exists T (Int: @grammar _ T) St,
-        forall (w: @word Tt),
-          dfa_language dfa w /\ language G S (to_phrase w) <->
-          language Int St (to_phrase w).
+    Theorem grammar_of_intersection_exists:
+      exists (NewNonterminal: Type) (IntersectionGrammar: @grammar Terminal NewNonterminal) St,
+        forall word,
+          dfa_language dfa word /\ language G S (to_phrase word) <->
+          language IntersectionGrammar St (to_phrase word).
     Proof.
       have Alt: forall n, n == 0 \/ n > 0.
       { by move => m; case m; [left|right]. }
-      move: (Alt n) => [/eqP ZERO | POS]; clear Alt.
-      { exfalso; subst n.
+      move: (Alt number_of_states) => [/eqP ZERO | POS]; clear Alt.
+      { exfalso; subst number_of_states.
         destruct dfa.
         have C0 := case0 (fun _ => false).
           by apply C0 in start0.
       } 
       intros.
-      set (NG := @normalize Tt Vt _ _ TToNat UToNat NatToU bijection G).
+      set (NG := @normalize Terminal Nonterminal _ _ TToNat UToNat NatToU bijection G).
       set (SDFAS := split_dfa dfa).
       set (TRS :=
              map (fun s_dfa =>
                     (V (s_start s_dfa, S, s_final s_dfa), @convert_grammar _ _ _ NG s_dfa)) SDFAS).
-      set (I := (V (Union.start (t n * @var Vt * t n)), Union.grammar_union TRS)).
+      set (I := (V (Union.start (t number_of_states * @var Nonterminal * t number_of_states)), Union.grammar_union TRS)).
       set (I1 := fst I).
       set (I2 := snd I).
       have ALT:
-        (@dfa_language DfaState Tt dfa [] /\ language G S []) \/
-        (~ @dfa_language DfaState Tt dfa [] \/ ~ language G S []).
+        (@dfa_language DfaState Terminal dfa [] /\ language G S []) \/
+        (~ @dfa_language DfaState Terminal dfa [] \/ ~ language G S []).
       { have DECDFA: {dfa_language dfa []} + {~ dfa_language dfa []}.
         { apply list_in_dec.
           unfold DfaState.
@@ -977,11 +931,12 @@ Module Intersection.
       }
       move: ALT => [EPS|EPS].
       { set (II :=
-               (V (Union.start (Union.labeled_Vt (t n * @var Vt * t n))),
-                @Union.grammar_union Tt (Union.labeled_Vt (t n * var * t n)) [:: (I1, [R I1 []]); (I1, I2)])).
+               (V (Union.start (Union.labeled_Vt (t number_of_states * @var Nonterminal * t number_of_states))),
+                @Union.grammar_union Terminal (Union.labeled_Vt (t number_of_states * var * t number_of_states))
+                                     [:: (I1, [R I1 []]); (I1, I2)])).
         set (II1 := fst II).
         set (II2 := snd II).       
-        exists ((Union.labeled_Vt (Union.labeled_Vt (t n * @var Vt * t n)))), II2, II1.
+        exists ((Union.labeled_Vt (Union.labeled_Vt (t number_of_states * @var Nonterminal * t number_of_states)))), II2, II1.
         intros w.
         case: w => [|].
         { split; intros.
@@ -1000,13 +955,13 @@ Module Intersection.
           split; last by right.
           { apply H_correct_split in DL.
             move: DL => [s_dfa [EL LANG]].
-            have MF := @main_forward Tt Vt n NG _ _ _ s_dfa S (a::w).
+            have MF := @main_forward Terminal Nonterminal number_of_states NG _ _ _ s_dfa S (a::w).
             feed_n 4 MF; try done.
             { by apply chomsky_normalform. }
             { intros; repeat split.
-              - destruct n; [by done | by apply F1].
+              - destruct number_of_states; [by done | by apply F1].
               - by done.
-              - destruct n; [by done | by apply F1].
+              - destruct number_of_states; [by done | by apply F1].
             }
             { by split; last apply language_normalform. }
             eapply Union.correct_union_2.
@@ -1027,7 +982,7 @@ Module Intersection.
             { exfalso.
               inversion EL; subst gr; subst v; clear EL.
               move: LANG => [DER _].
-                by apply Fact1 in DER. }
+                by apply non_epsilon_is_not_derivable_in_epsilon_grammar in DER. }
             { inversion EL; subst gr; subst v; clear EL.
               have CORRECT := Union.correct_union_2 _ (a::w).
               apply CORRECT in LANG.
@@ -1036,7 +991,7 @@ Module Intersection.
               unfold TRS in EL; apply in_map_iff in EL.
               move: EL => [s_dfa [EQ EL]].
               inversion EQ; subst gr; subst v; clear EQ.
-              have MB := @main_backward Tt Vt n NG _ _ _ s_dfa (a::w) S.
+              have MB := @main_backward Terminal Nonterminal number_of_states NG _ _ _ s_dfa S (a::w).
               feed_n 4 MB; try done.
               { by apply chomsky_normalform. }
               { by intros; apply NatToU. }
@@ -1054,11 +1009,9 @@ Module Intersection.
         } 
       }
       {
-
-        exists (((Union.labeled_Vt (t n * @var Vt * t n)))), I2, I1.
-        
+        exists (((Union.labeled_Vt (t number_of_states * @var Nonterminal * t number_of_states)))), I2, I1.
         intros w.
-       case: w => [|].
+        case: w => [ | ].
         { 
           split; intros.
           - exfalso.
@@ -1072,7 +1025,7 @@ Module Intersection.
             unfold TRS in EL; apply in_map_iff in EL.
             move: EL => [s_dfa [EQ EL]].
             inversion EQ; subst v; subst gr; clear EQ.
-            have MB := @main_backward Tt Vt n NG _ _ _ s_dfa ([]) S.
+            have MB := @main_backward Terminal Nonterminal number_of_states NG _ _ _ s_dfa S ([]).
             feed_n 4 MB; try done.
             { by apply chomsky_normalform. }
             { by intros; apply NatToU. }
@@ -1080,20 +1033,20 @@ Module Intersection.
             move: MB => [DLANG LANG].
             simpl in LANG.
             unfold NG in LANG.
-              by apply lflfl in LANG.
+              by apply epsilon_is_not_derivable_in_normalized_grammar in LANG.
         }
         { 
           intros a w.
           split; [move => [DL GL]| move => IL].
           { apply H_correct_split in DL.
             move: DL => [s_dfa [EL LANG]].
-            have MF := @main_forward Tt Vt n NG _ _ _ s_dfa S (a::w).
+            have MF := @main_forward Terminal Nonterminal number_of_states NG _ _ _ s_dfa S (a::w).
             feed_n 4 MF; try done.
             { by apply chomsky_normalform. }
             { intros; repeat split.
-              - destruct n; [by done | by apply F1].
+              - destruct number_of_states; [by done | by apply F1].
               - by done.
-              - destruct n; [by done | by apply F1].
+              - destruct number_of_states; [by done | by apply F1].
             }
             { by split; last apply language_normalform. }
             eapply Union.correct_union_2.
@@ -1104,8 +1057,7 @@ Module Intersection.
               apply in_map_iff.
               exists s_dfa; split; by done.
           }
-          { 
-            intros.
+          { intros.
             unfold I2, I1, I in IL.
             eapply Union.correct_union_2 in IL.
             move: IL => [[gr v] [LANG EL]]; simpl in *.
@@ -1113,7 +1065,7 @@ Module Intersection.
             apply in_map_iff in EL.
             move: EL => [s_dfa [EQ EL]].
             inversion EQ; subst gr; subst v; clear EQ.
-            have MB := @main_backward Tt Vt n NG _ _ _ s_dfa (a::w) S.
+            have MB := @main_backward Terminal Nonterminal number_of_states NG _ _ _ s_dfa S (a::w).
             feed_n 4 MB; try done.
             { by apply chomsky_normalform. }
             { by intros; apply NatToU. }
@@ -1128,9 +1080,9 @@ Module Intersection.
           }
         }
       } 
-    Qed.
+    Qed. 
     
-  End Main3.
-   
+  End Main.
+  
 End Intersection.
 
